

Lever Arm Equations

$$\vec{L}^E = C_B^E \vec{L}^B$$

$$\dot{\vec{L}}^E = \dot{C}_B^E \vec{L}^B + C_B^E \dot{\vec{L}}^B$$

$\dot{C}_B^E = C_B^E (\omega_{EB}^B \times) \rightarrow \dot{C}_B^E = (\omega_{EB}^E \times) C_B^E$

$$\dot{\vec{L}}^E = (\omega_{EB}^E \times) (C_B^E \vec{L}^B) = (\omega_{EB}^E \times \vec{L}^E)$$

$$\dot{\vec{L}}^E = (\omega_{EB}^E \times \vec{L}^E)$$

$$\ddot{\vec{L}}^E = (\dot{\omega}_{EB}^E \times \vec{L}^E) + (\omega_{EB}^E \times \dot{\vec{L}}^E)$$

$\dot{\omega}_{EB}^E = \dot{\omega}_{EP}^E + \dot{\omega}_{PB}^E$ SMALL ~ a/Re

P = Platform frame (local level tangent frame) computed

$$\ddot{\vec{L}}^E = \dot{\omega}_{PB}^E \times \vec{L}^E + \omega_{EB}^E \times (\omega_{EB}^E \times \vec{L}^E)$$

$\vec{A} \times \vec{B} \times \vec{C} = \vec{B}(\vec{A} \cdot \vec{C}) - \vec{C}(\vec{A} \cdot \vec{B})$

$$\omega \times \omega \times L = \omega(\omega \cdot L) - L(\omega \cdot \omega) = \vec{\omega}_{EB}^E (\omega_{EB}^E \cdot \vec{L}^E) - \omega_{EB}^{E\,2} \vec{L}^E$$
$$\ddot{\vec{L}}^E = \dot{\omega}_{PB}^E \times \vec{L}^E + \vec{\omega}_{EB}^E (\omega_{EB}^E \cdot \vec{L}^E) - (\omega_{EB}^E)^2 \vec{L}^E$$

$$\ddot{\vec{L}}^E = \vec{\dot{\omega}}_{PB}^E \times \vec{L}^E + \vec{\omega}_{EB}^E (\omega_{EB}^E \cdot \vec{L}^E) - (\omega_{EB}^E)^2 \vec{L}^E$$